pulse/ulib/experimental/Steel.HigherReference.fsti
@@ -78,3 +78,11 @@ val recall (#a:Type u#1) (#q:perm) (#p:Preorder.preorder a) (#fact:property a)
            (r:reference a p) (v:(Ghost.erased a))
   : SteelT unit (pts_to_ref r q v `star` pure (witnessed r fact))
                 (fun _ -> pts_to_ref r q v `star` pure (fact v))
+
+val lem_star_pure (p : hprop) (f: prop)
+  : Lemma (requires f)
+          (ensures (p `equiv` (p `star` pure f)))
+
+val lem_interp_star_pure (p: hprop) (f: prop) (m: mem)
+  : Lemma (requires (interp (p `star` pure f)) m)
+          (ensures f)
